\documentclass{amsart}
\usepackage[ocgcolorlinks,linktoc=all]{hyperref}
\hypersetup{citecolor=blue,linkcolor=red}
\newtheorem{theorem}{Theorem}
\newtheorem*{thmA}{Theorem}
\newtheorem*{thmB}{Theorem}
\newtheorem*{rem}{Remark}
\newtheorem*{thmmain}{Theorem}
\newtheorem{lemma}[theorem]{Lemma}
\newtheorem{proposition}[theorem]{Proposition}
\newtheorem*{propmain}{Proposition}
\newtheorem{corollary}[theorem]{Corollary}
\theoremstyle{definition}
\newtheorem{definition}[theorem]{Definition}
\newtheorem{example}[theorem]{Example}
\newtheorem{xca}[theorem]{Exercise}

\theoremstyle{remark}
\newtheorem{remark}[theorem]{Remark}

\newcommand{\abs}[1]{\lvert#1\rvert}
\numberwithin{equation}{section}

\newcommand{\blankbox}[2]{%
  \parbox{\columnwidth}{\centering
    \setlength{\fboxsep}{0pt}%
    \fbox{\raisebox{0pt}[#2]{\hspace{#1}}}%
  }%
}

%%%%%%%%%%%%%%%%%%%%%%%%%%%%%%%%%%%%%%
%%%Julian's shortcuts
\usepackage{cleveref}
\crefname{lemma}{Lemma}{Lemmata}

%Symbols
\renewcommand{\~}{\tilde}
\renewcommand{\-}{\bar}
\newcommand{\bs}{\backslash}
\newcommand{\cn}{\colon}
\newcommand{\sub}{\subset}

\newcommand{\N}{\mathbb{N}}
\newcommand{\R}{\mathbb{R}}
\newcommand{\Z}{\mathbb{Z}}
\renewcommand{\S}{\mathbb{S}}
\renewcommand{\H}{\mathbb{H}}
\newcommand{\C}{\mathbb{C}}
\newcommand{\K}{\mathbb{K}}
\newcommand{\Di}{\mathbb{D}}
\newcommand{\B}{\mathbb{B}}
\newcommand{\8}{\infty}

%Greek letters
\renewcommand{\a}{\alpha}
\renewcommand{\b}{\beta}
\newcommand{\g}{\gamma}
\renewcommand{\d}{\delta}
\newcommand{\e}{\epsilon}
\renewcommand{\k}{\kappa}
\renewcommand{\l}{\lambda}
\renewcommand{\o}{\omega}
\renewcommand{\t}{\theta}
\newcommand{\s}{\sigma}
\newcommand{\p}{\varphi}
\newcommand{\z}{\zeta}
\newcommand{\vt}{\vartheta}
\renewcommand{\O}{\Omega}
\newcommand{\D}{\Delta}
\newcommand{\G}{\Gamma}
\newcommand{\T}{\Theta}
\renewcommand{\L}{\Lambda}

%Mathematical operators
\newcommand{\del}{\partial}
\newcommand{\inpr}[2]{\left\langle #1,#2 \right\rangle}
\newcommand{\fr}[2]{\frac{#1}{#2}}
\newcommand{\x}{\times}



%Environments
\newcommand{\Theo}[3]{\begin{#1}\label{#2} #3 \end{#1}}
\newcommand{\pf}[1]{\begin{proof} #1 \end{proof}}
\newcommand{\eq}[1]{\begin{equation}\begin{alignedat}{2} #1 \end{alignedat}\end{equation}}
\newcommand{\br}[1]{\left(#1\right)}



%Logical symbols
\newcommand{\Ra}{\Rightarrow}
\newcommand{\ra}{\rightarrow}
\newcommand{\hra}{\hookrightarrow}
\newcommand{\mt}{\mapsto}

%Fonts
\newcommand{\mc}{\mathcal}
\renewcommand{\it}{\textit}
\newcommand{\mrm}{\mathrm}

%Spacing
\newcommand{\hp}{\hphantom}
%%%%%%%%%%%%%%%%%%%%%%%%%%%%%%%%%%%%%%%%%%%%%%%%%%
%%%%%%%%%%%%%%%%%%%%%%%%%%%%%%%%%%%%%%%%%%%%%%%%%






\begin{document}

\title[]
 {Harnack estimates for curvature flow equations in space forms}

\curraddr{}
\email{}
\date{\today}

\dedicatory{}
\subjclass[2010]{}
\keywords{}

\begin{abstract}
%We prove differential Harnack inequalities for weakly convex hypersurfaces on the unit sphere shrinking by positive powers of homogeneous degree one, inverse-concave functions of principal curvatures, $f^{\alpha}>0,~\alpha\geq 1$ . As an application, we prove that the only convex, ancient solutions of curvature flows with $f$ concave and inverse-concave velocities are shrinking geodesic spheres.
\end{abstract}

\maketitle

\section{Evolution equations}
We consider the flow equation
\eq{\dot{x}=-\p(f)\nu}
in a space form of sectional curvature $\l,$ where $f$ is a 1-homogeneous, concave and inverse concave curvature function. Let
\eq{\p^{ij}=\fr{\del\p}{\del h_{ij}}}
and for a tensor $T,$
\eq{\Box T=\p^{ij}T_{;ij},}
where $_{;i}$ denotes differentiation $\nabla_{i}$ with respect to the L\'evi-Civita connection $\nabla.$
The evolution equations in the following lemma are standard, compare \cite[p.~94-95]{Gerhardt:/2006}. \cref{EvInvh} can easily be derived from \cref{EvInvg} and \cref{EvCovh}, also compare the formula \cite[eq.~(6.17)]{Gerhardt:01/1996}.
\Theo{lemma}{Eveq1}{

\eq{\label{Evg}\dot{g}_{ij}=-2\p h_{ij}.}
\eq{\label{EvInvg}\dot{g}^{ij}=2\p h^{ij}.}
\eq{\label{EvMixedh}\dot{h}^{j}_{i}={\p_{;i}}^{j}+\p h^{j}_{k}h^{k}_{i}+\l\p\d^{j}_{i}.}
\eq{\label{EvCovh}\dot{h}_{ij}=\p_{;ij}-\p h^{k}_{i}h_{kj}+\l\p g_{ij}.}
\eq{\label{Evphi}\dot{\p}-\Box\p=\p^{ij}h_{ik}h^{k}_{j}\p+\l\p^{ij}g_{ij}\p.}
\eq{\label{EvInvh}\dot{b}^{ij}-\Box b^{ij}&=-\p^{rs}h_{rk}h^{k}_{s}b^{ij}+\br{\p'f+\p}g^{ij}-\l\br{\p'f+\p}b^{ir}b^{j}_{r}+\l\p^{kl}g_{kl}b^{ij}\\
						&\hp{=}-\br{2b^{lq}\p^{kp}+\p^{kl,pq}}b^{ir}b^{js}h_{kl;r}h_{pq;s},}
						where $(b^{ij})$ denotes the inverse of $(h_{ij}).$
}

\Theo{lemma}{EvGamma}{
The Christoffel symbols evolve according to
\eq{\dot{\G}^{k}_{ij}=-\p g^{kl}h_{ij;l}-g^{kl}\p_{;j}h_{li}-g^{kl}\p_{;i}h_{lj}+g^{kl}\p_{;l}h_{ij}.}
}

\pf{
We have
\eq{\G^{k}_{ij}=\fr{1}{2}g^{kl}\br{g_{il,j}+g_{jl,i}-g_{ij,l}},}
where $_{,i}$ denotes partial differentiation with respect to $\xi^{i}$ in a coordinate system $(\xi^{i}).$
Since $\dot{\G}^{k}_{ij}$ is a tensor, we may a priorily consider normal coordinates in a given point. Then, using the Codazzi equations,
\eq{\dot{\G}^{k}_{ij}&=\fr{1}{2}g^{kl}\br{\dot{g}_{il,j}+\dot{g}_{jl,i}-\dot{g}_{ij,l}}\\
				&=-\p g^{kl}h_{ij;l}-g^{kl}\p_{;j}h_{il}-g^{kl}\p_{;i}h_{lj}+g^{kl}\p_{;l}h_{ij}.}
}



\Theo{lemma}{deltBox}{
There holds
\eq{\br{\del_{t}\Box-\Box\del_{t}}\p&=2\p^{ij}h^{k}_{i}\br{\p_{;kj}\p+\p_{;k}\p_{;j}}+\br{\p-\p^{ij}h_{ij}}|\nabla\p|^{2}\\
					&\hp{=}+\p^{ij,rs}\p_{;ij}\br{\p_{;rs}+\p h_{rm}h^{m}_{s}+\l\p g_{rs}}.}
}


\pf{Considering the curvature function $\p$ to depend on $(h_{ij})$ and $(g_{ij}),$
\eq{\p=\p(h_{ij},g_{ij}),}
we denote
\eq{\p^{ij}=\fr{\del \p}{\del h_{ij}},\quad \p^{ij,kl}=\fr{\del^{2}\p}{\del h_{ij}\del h_{kl}},}
which are tensors, in particular we have
\eq{\p^{i}_{j}\equiv \fr{\del \p}{\del h^{j}_{i}}=\p^{ik}g_{kj}.}
Furthermore we have
\eq{\fr{\del\p}{\del g_{ij}}=\p^{l}_{k}\fr{\del h^{k}_{l}}{\del g_{ij}}=-\p^{l}_{k}g^{ki}g^{rj}h_{rl}=-\p^{li}h^{j}_{l}.}
Thus
\eq{\label{deltBox1}\del_{t}\p^{ij}&=\p^{ij,kl}\dot{h}_{kl}+\fr{\del\p^{ij}}{\del g_{kl}}\dot{g}_{kl}\\
			&=\p^{ij,kl}\br{\dot{h}_{kl}+2\p h_{lm}h^{m}_{k}}+2\p\p^{jk}g^{li}h_{kl}\\
			&=\p^{ij,kl}\br{\dot{h}_{kl}+2\p h_{lm}h^{m}_{k}}+2\p\p^{jk}h^{i}_{k}.}
We obtain from \cref{EvGamma},
\eq{\br{\del_{t}\Box-\Box\del_{t}}\p&=\br{\del_{t}\p^{ij}}\p_{;ij}+\p^{ij}\br{\del_{t}\p_{;ij}-\dot{\p}_{;ij}}\\
							&=\br{\del_{t}\p^{ij}}\p_{;ij}-\p^{ij}\dot{\G}^{k}_{ij}\p_{;k}\\
							&=2\p h^{i}_{k}\p^{kj}\p_{;ij}+\p^{ij,rs}\br{\dot{h}_{rs}+2\p h_{rm}h^{m}_{s}}\p_{;ij}\\
							&\hp{=}+\p\p^{ij}h_{ij;l}g^{kl}\p_{;k}+2\p^{ij}g^{kl}h_{li}\p_{;j}\p_{;k}-\p^{ij}h_{ij}g^{kl}\p_{;l}\p_{;k}. }
	}	

\Theo{lemma}{Evbeta}{
The quantity 
\eq{\b=\dot{\p}-\l\p^{ij}g_{ij}\p=\Box\p+\p^{ij}h_{ik}h^{k}_{j}\p.}
satisfies
\eq{\br{\del_{t}-\Box}\b&=\p^{ij}h_{ik}h^{k}_{j}\b+2\p^{ij}h^{k}_{i}\br{2\p_{;kj}\p+\p_{;k}\p_{;j}+h^{s}_{j}h_{sk}\p^{2}}\\
				&\hp{=}+\br{\p-\p^{ij}h_{ij}}|\nabla\p|^{2}\\
				&\hp{=}+\p^{ij,kl}\br{\p_{;ij}+h_{ip}h^{p}_{j}\p}\br{\p_{;kl}+h^{m}_{k}h_{ml}\p}\\
				&\hp{=}+\l\p^{ij}g_{ij}\b+2\l\p^{rs}\br{\p^{ij}g_{ij}}_{;r}\p_{;s}+\l\Box\br{\p^{ij}g_{ij}}\p\\
				&\hp{=}+\l\p^{ij,rs}g_{rs}\br{\p_{;ij}\p+h_{ik}h^{k}_{j}\p^{2}}+2\l\p^{ij}h_{ij}\p^{2}.}
}

\pf{We will need the following auxillary calculation, where we use \cref{deltBox1}.
\eq{\del_{t}\br{\p^{ij}h_{ik}h^{k}_{j}}&=\del_{t}\p^{ij}h_{ik}h^{k}_{j}+\p^{ij}\dot{h}_{ik}h^{k}_{j}+\p^{ij}h_{ik}\dot{h}^{k}_{j}\\
				&=\p^{ij,kl}\br{\dot{h}_{kl}+2\p h_{kr}h^{r}_{l}}h_{ir}h^{r}_{j}+2\p\p^{jk}h^{i}_{k}h_{ir}h^{r}_{j}\\
				&\hp{=}+\p^{ij}\br{\p_{;ik}-\p h^{r}_{i}h_{rk}+\l\p g_{ik}}h^{k}_{j}\\
				&\hp{=}+\p^{ij}\br{{\p_{;j}}^{k}+\p h^{k}_{r}h^{r}_{j}+\l\p\d^{k}_{j}}h_{ik}\\
				&=\p^{ij,kl}\br{\p_{;kl}+\p h^{r}_{k}h_{rl}+\l\p g_{kl}}h_{is}h^{s}_{j}+2\p\p^{jk}h^{i}_{k}h_{ir}h^{r}_{j}\\
				&\hp{=}+2\p^{ij}h^{k}_{i}\p_{;jk}+2\l\p^{ij}h_{ij}\p.}

 We use \cref{deltBox} to compute
\eq{\br{\del_{t}-\Box}\b&=\del_{t}\Box\p+\del_{t}\br{\p^{ij}h_{ik}h^{k}_{j}\p}-\Box\Box\p-\Box\br{\p^{ij}h_{ik}h^{k}_{j}\p}\\
			&=\Box\br{\l\p^{ij}g_{ij}\p}+2\p^{ij}h^{k}_{i}\br{\p_{;kj}\p+\p_{;k}\p_{;j}}+\br{\p-\p^{ij}h_{ij}}|\nabla\p|^{2}\\
					&\hp{=}+\p^{ij,rs}\p_{;ij}\br{\p_{;rs}+\p h_{rm}h^{m}_{s}+\l\p g_{rs}}+\del_{t}\br{\p^{ij}h_{ik}h^{k}_{j}\p}\\
			&=\l\p^{ij}g_{ij}\b-\l\p^{kl}g_{kl}\p^{ij}h_{ir}h^{r}_{j}\p+2\l\p^{rs}\br{\p^{ij}g_{ij}}_{;r}\p_{;s}\\
			&\hp{=}+\l\Box\br{\p^{ij}g_{ij}}\p+2\p^{ij}h^{k}_{i}\br{\p_{;kj}\p+\p_{;k}\p_{;j}}\\
			&\hp{=}+\br{\p-\p^{ij}h_{ij}}|\nabla\p|^{2}+\p^{ij,rs}\p_{;ij}\br{\p_{;rs}+\p h_{rm}h^{m}_{s}+\l\p g_{rs}}\\
			&\hp{=}+\p^{ij}h_{ik}h^{k}_{j}\b+\l\p^{ij}h_{ik}h^{k}_{j}\p^{rs}g_{rs}\p+\del_{t}\br{\p^{ij}h_{ik}h^{k}_{j}}\p\\
			&=\p^{ij}h_{ik}h^{k}_{j}\b+\l\p^{ij}g_{ij}\b+2\l\p^{rs}\br{\p^{ij}g_{ij}}_{;r}\p_{;s}\\
			&\hp{=}+\l\Box\br{\p^{ij}g_{ij}}\p+2\p^{ij}h^{k}_{i}\br{\p_{;kj}\p+\p_{;k}\p_{;j}}	\\
			&\hp{=}+\br{\p-\p^{ij}h_{ij}}|\nabla\p|^{2}+\p^{ij,rs}\p_{;ij}\br{\p_{;rs}+\p h_{rm}h^{m}_{s}+\l\p g_{rs}}\\
			&\hp{=}+\p^{ij,kl}\br{\p_{;kl}+\p h^{r}_{k}h_{rl}+\l\p g_{kl}}h_{is}h^{s}_{j}\p+2\p^{jk}h^{i}_{k}h_{ir}h^{r}_{j}\p^{2}\\
				&\hp{=}+2\p^{ij}h^{k}_{i}\p_{;jk}\p+2\l\p^{ij}h_{ij}\p^{2}.}
}

\Theo{lemma}{gradBox}{
For every smooth function $F$  there holds
\eq{\br{\Box F}_{;i}-\Box F_{;i}&=\p^{kl,rs}h_{rs;i}F_{;kl}+\l\p^{kl}g_{ki}F_{;l}-\l\p^{kl}g_{kl}F_{;i}\\
					&\hp{=}+\p^{kl}h^{m}_{l}h_{ki}F_{;m}-\p^{kl}h_{kl}h^{m}_{i}F_{;m}.}
}

\pf{
From the Ricci identities we obtain
\eq{\br{\p^{kl}F_{;kl}}_{;i}-\p^{kl}F_{;ikl}=\p^{kl,rs}h_{rs;i}F_{;kl}+\p^{kl}{R^{m}}_{kli}F_{;m}}
and from the Gauss equation we obtain
\eq{\p^{kl}{R^{m}}_{kli}F_{;m}=\l\p^{kl}g_{ki}F_{;l}-\l\p^{kl}g_{kl}F_{;i}+\p^{kl}h^{m}_{l}h_{ki}F_{;m}-\p^{kl}h_{kl}h^{m}_{i}F_{;m}.}
}

\Theo{lemma}{Evgradphi}{
There holds
\eq{\br{\del_{t}-\Box}\p_{;i}&=\br{\p^{kl}h_{kr}h^{r}_{l}\p}_{;i}+\l\p^{kl}\p_{;l}g_{ki}+\l\p^{kl,rs}h_{rs;i}g_{kl}\p\\
				&\hp{=}+\p^{kl,rs}h_{rs;i}\p_{;kl}+\br{\p^{kl}h^{m}_{l}h_{ki}-\p^{kl}h_{kl}h^{m}_{i}}\p_{;m}.}
}

\pf{
\eq{\del_{t}\p_{;i}-\Box\p_{;i}&=\br{\Box\p}_{;i}+\br{\p^{kl}h_{rk}h^{r}_{l}\p}_{;i}+\l\br{\p^{kl}g_{kl}\p}_{;i}\\
					&\hp{=}-\br{\Box\p}_{;i}+\p^{kl,rs}h_{rs;i}\p_{;kl}+\l\p^{kl}g_{ki}\p_{;l}-\l\p^{kl}g_{kl}\p_{;i}\\
					&\hp{=}+\p^{kl}h^{m}_{l}h_{ki}\p_{;m}-\p^{kl}h_{kl}h^{m}_{i}\p_{;m}\\
					&=\br{\p^{kl}h_{rk}h^{r}_{l}\p}_{;i}+\l\p^{kl,rs}h_{rs;i}g_{kl}\p+\p^{kl,rs}h_{rs;i}\p_{;kl}\\
					&\hp{=}+\l\p^{kl}g_{ki}\p_{;l}+\br{\p^{kl}h^{m}_{l}h_{ki}-\p^{kl}h_{kl}h^{m}_{i}}\p_{;m}.}
}

\Theo{lemma}{Evtheta}{
The quantity $\t=b^{ij}\p_{;i}\p_{;j}$ satisfies
\eq{\br{\del_{t}-\Box}\t&=\p^{rs}h_{rk}h^{k}_{s}\t-\br{2b^{lq}\p^{kp}+\p^{kl,pq}}b^{ir}b^{js}\p_{;i}\p_{j}h_{kl;r}h_{pq;s}\\
							&\hp{=}+\br{\p'f+\p-2\p^{kl}h_{kl}}|\nabla\p|^{2}+2\p^{jl}h^{m}_{l}\p_{;m}\p_{;j}\\
							&\hp{=}+2b^{ij}\p^{kl,rs}h_{rs;i}\p_{;j}\br{\p_{;kl}+h_{rk}h^{r}_{l}\p}+4b^{ij}\p^{kl}h_{rk;i}h^{r}_{l}\p_{;j}\p\\
							&\hp{=}+4\p^{rs}b^{ip}b^{jq}h_{pq;r}\p_{;is}\p_{;j}-2b^{ij}\p^{rs}\p_{;ir}\p_{;js}\\
							&\hp{=}-\l\br{\p'f+\p}b^{ir}b^{j}_{r}\p_{;i}\p_{;j}+\l\p^{kl}g_{kl}\t+2\l b^{j}_{k}\p^{kl}\p_{;l}\p_{;j}\\
							&\hp{=}+2\l b^{ij}\p^{kl,rs}h_{rs;i}\p_{;j}g_{kl}\p.}
}

\pf{
\eq{\br{\del_{t}-\Box}\t&=\br{\dot{b}^{ij}-\Box b^{ij}}\p_{;i}\p_{;j}+2b^{ij}\br{\dot{\p}_{;i}-\Box\p_{;i}}\p_{;j}\\
							&\hp{=}-4\p^{rs}{b^{ij}}_{;r}\p_{;is}\p_{;j}-2b^{ij}\p^{rs}\p_{;ir}\p_{;js}\\
							&=-\p^{rs}h_{rk}h^{k}_{s}\t+\br{\p'f+\p}|\nabla\p|^{2}-\l\br{\p'f+\p}b^{ir}b^{j}_{r}\p_{;i}\p_{;j}\\
							&\hp{=}+\l\p^{kl}g_{kl}\t-\br{2b^{lq}\p^{kp}+\p^{kl,pq}}b^{ir}b^{js}\p_{;i}\p_{;j}h_{kl;r}h_{pq;s}\\
							&\hp{=}+2\p^{kl}h_{rk}h^{r}_{l}\t+2b^{ij}\br{\p^{kl}h_{rk}h^{r}_{l}}_{;i}\p_{;j}\p+2b^{ij}\p^{kl,rs}h_{rs;i}\p_{;j}\p_{;kl}\\
							&\hp{=}+2b^{ij}\br{\p^{kl}h^{m}_{l}h_{ki}-\p^{kl}h_{kl}h^{m}_{i}}\p_{;m}\p_{;j}\\
							&\hp{=}+2\l b^{ij}\p^{kl,rs}h_{rs;i}\p_{;j}g_{kl}\p+2\l b^{j}_{k}\p^{kl}\p_{;l}\p_{;j}\\
							&\hp{=}-4\p^{rs}{b^{ij}}_{;r}\p_{;is}\p_{;j}-2b^{ij}\p^{rs}\p_{;ir}\p_{;js}\\
							&=\p^{rs}h_{rk}h^{k}_{s}\t-\br{2b^{lq}\p^{kp}+\p^{kl,pq}}b^{ir}b^{js}\p_{;i}\p_{;j}h_{kl;r}h_{pq;s}\\
							&\hp{=}+\br{\p'f+\p}|\nabla\p|^{2}+2\p^{jl}h^{m}_{l}\p_{;m}\p_{;j}-2\p^{kl}h_{kl}|\nabla\p|^{2}\\
							&\hp{=}+2b^{ij}\p^{kl,rs}h_{rs;i}\p_{;j}\br{\p_{;kl}+h_{rk}h^{r}_{l}\p}+4b^{ij}\p^{kl}h_{rk;i}h^{r}_{l}\p_{;j}\p\\
							&\hp{=}-4\p^{rs}{b^{ij}}_{;r}\p_{;is}\p_{;j}-2b^{ij}\p^{rs}\p_{;ir}\p_{;js}\\
							&\hp{=}-\l\br{\p'f+\p}b^{ir}b^{j}_{r}\p_{;i}\p_{;j}+\l\p^{kl}g_{kl}\t+2\l b^{j}_{k}\p^{kl}\p_{;l}\p_{;j}\\
							&\hp{=}+2\l b^{ij}\p^{kl,rs}h_{rs;i}\p_{;j}g_{kl}\p.}
}

\Theo{lemma}{Evchi}{
Let $\d\neq 0.$ The quantity 
\eq{\chi=t(\b-\t)+\d\p}
satisfies
\eq{\dot{\chi}-\Box\chi&=\br{\fr{\b-\t}{\d\p}+\p^{ij}h_{ik}h^{k}_{j}+\l\p^{ij}g_{ij}}\chi\\
				&\hp{=}+t\br{\p^{ij,kl}+2b^{il}\p^{jk}-\fr{\p^{ij}\p^{kl}}{\d\p}}\eta_{ij}\eta_{kl}+t\l R,}
where
\eq{\eta_{ij}=\p_{;ij}-b^{rs}h_{ij;r}\p_{;s}+h_{ip}h^{p}_{j}\p}
and 
\eq{R&=2\p^{rs}\br{\p^{ij}g_{ij}}_{;r}\p_{;s}+\Box\br{\p^{ij}g_{ij}}\p\\
				&\hp{=}+\p^{kl,rs}g_{rs}\br{\p_{;kl}\p+h_{kr}h^{r}_{l}\p^{2}-2b^{ij}h_{kl;i}\p_{;j}\p}+2\p^{ij}h_{ij}\p^{2}\\
				&\hp{=}+\br{\p'f+\p}b^{ir}b^{j}_{r}\p_{;i}\p_{;j}-2 b^{j}_{k}\p^{kl}\p_{;l}\p_{;j}.
}
}
	
\pf{
\eq{\dot\chi&-\Box\chi=\b-\t+t\br{\br{\del_{t}-\Box}\br{\b-\t}}+\d\br{\dot\p-\Box\p}\\
				&=\b-\t+\d\p^{ij}h_{ik}h^{k}_{j}\p+\d\l\p^{ij}g_{ij}\p\\
				&\hp{=}+t\Big(\p^{ij}h_{ik}h^{k}_{j}\br{\b-\t}+\br{\p^{ij}h_{ij}-\p'f}|\nabla\p|^{2}\\
				&\hp{=}+\p^{ij,kl}\br{\p_{;ij}+h_{ip}h^{p}_{j}\p}\br{\p_{;kl}+h^{m}_{k}h_{ml}\p}\\
				&\hp{=}+\p^{ij,kl}b^{pr}b^{sq}\p_{;p}\p_{;q}h_{ij;r}h_{kl;s}-2\p^{ij,kl}b^{rs}h_{kl;r}\p_{;s}\br{\p_{;ij}+h_{ip}h^{p}_{j}\p}\\
				&\hp{=}+2\p^{ik}h^{r}_{i}\br{2\p_{;rk}\p+h^{s}_{k}h_{sr}\p^{2}}+2b^{il}\p^{jk}b^{pr}b^{qs}\p_{;p}\p_{;q}h_{kl;r}h_{ij;s}\\
				&\hp{=}-4b^{il}\p^{jk}h_{rk;i}h^{r}_{j}\p_{;l}\p-4\p^{jk}b^{il}b^{pq}h_{lj;q}\p_{;ik}\p_{;p}+2b^{il}\p^{jk}\p_{;ij}\p_{;lk}\\
				&\hp{=}+\l\p^{ij}g_{ij}\br{\b-\t}+2\l\p^{rs}\br{\p^{ij}g_{ij}}_{;r}\p_{;s}+\l\Box\br{\p^{ij}g_{ij}}\p\\
				&\hp{=}+\l\p^{kl,rs}g_{rs}\br{\p_{;kl}\p+h_{kr}h^{r}_{l}\p^{2}-2b^{ij}h_{kl;i}\p_{;j}\p}+2\l\p^{ij}h_{ij}\p^{2}\\
				&\hp{=}+\l\br{\p'f+\p}b^{ir}b^{j}_{r}\p_{;i}\p_{;j}-2\l b^{j}_{k}\p^{kl}\p_{;l}\p_{;j}\Big)\\
				&=\b-\t+\br{\p^{ij}h_{ik}h^{k}_{j}+\l\p^{ij}g_{ij}}\chi+t\br{\p^{ij}h_{ij}-\p'f}|\nabla\p|^{2}\\
				&\hp{=}+t\p^{ij,kl}\br{\p_{;ij}-b^{rs}h_{ij;r}\p_{;s}+h_{ip}h^{p}_{j}\p}\br{\p_{;kl}-b^{mn}h_{kl;m}\p_{;n}+h_{kq}h^{q}_{l}\p}\\
				&\hp{=}+2tb^{il}\p^{jk}\br{\p_{;ij}-b^{rs}h_{ij;r}\p_{;s}+h_{ip}h^{p}_{j}\p}\br{\p_{;kl}-b^{mn}h_{kl;m}\p_{;n}+h_{kq}h^{q}_{l}\p}\\
				&\hp{=}+2t\l\p^{rs}\br{\p^{ij}g_{ij}}_{;r}\p_{;s}+t\l\Box\br{\p^{ij}g_{ij}}\p\\
				&\hp{=}+t\l\p^{kl,rs}g_{rs}\br{\p_{;kl}\p+h_{kr}h^{r}_{l}\p^{2}-2b^{ij}h_{kl;i}\p_{;j}\p}+2t\l\p^{ij}h_{ij}\p^{2}\\
				&\hp{=}+t\l\br{\p'f+\p}b^{ir}b^{j}_{r}\p_{;i}\p_{;j}-2t\l b^{j}_{k}\p^{kl}\p_{;l}\p_{;j}.
}
}			
	





\bibliographystyle{amsplain}
\bibliography{Bibliography.bib}


\end{document}
